CBOR.Pulse.Raw.Compare

src/cbor/pulse/raw/CBOR.Pulse.Raw.Compare.fst
@@ -239,7 +239,7 @@ fn cbor_compare_body
       let i1 = cbor_match_int_elim_value x1;
       let i2 = cbor_match_int_elim_value x2;
       impl_raw_uint64_compare () i1 i2
-    } else if (ty1 = cbor_major_type_byte_string || ty1 = cbor_major_type_byte_string) {
+    } else if (ty1 = cbor_major_type_byte_string || ty1 = cbor_major_type_text_string) {
       let i1 = cbor_match_string_elim_length x1;
       let i2 = cbor_match_string_elim_length x2;
       let c : I16.t = impl_raw_uint64_compare () i1 i2;
@@ -277,8 +277,37 @@ fn cbor_compare_body
         cbor_compare_array_eq (Array?.v v1) (Array?.v v2);
         let f64 : squash (SZ.fits_u64) = assume (SZ.fits_u64);
         let i1 = cbor_array_iterator_init f64 x1;
+        with p1' . assert (cbor_array_iterator_match p1' i1 (Array?.v v1));
+        unfold (cbor_array_iterator_match p1' i1 (Array?.v v1));
         let i2 = cbor_array_iterator_init f64 x2;
-        let res = lex_compare_iterator_peel_perm cbor_match cbor_serialized_array_iterator_match cbor_serialized_array_iterator_is_empty (cbor_serialized_array_iterator_next f64) cbor_compare (impl_compare_of_cbor_compare ih) () i1 i2;
+        with p2' . assert (cbor_array_iterator_match p2' i2 (Array?.v v2));
+        unfold (cbor_array_iterator_match p2' i2 (Array?.v v2));
+        let res = lex_compare_iterator_peel_perm cbor_match cbor_serialized_array_iterator_match cbor_serialized_array_iterator_is_empty (cbor_serialized_array_iterator_next f64) cbor_compare (impl_compare_of_cbor_compare ih) i1 i2;
+        fold (cbor_array_iterator_match p1' i1 (Array?.v v1));
+        fold (cbor_array_iterator_match p2' i2 (Array?.v v2));
+        Trade.elim _ (cbor_match p1 x1 v1);
+        Trade.elim _ (cbor_match p2 x2 v2);
+        res
+      } else {
+        c
+      }
+    } else if (ty1 = cbor_major_type_map) {
+      let len1 = cbor_match_map_get_length x1;
+      let len2 = cbor_match_map_get_length x2;
+      let c = impl_raw_uint64_compare () len1 len2;
+      if (c = 0s) {
+        // FIXME: add a case to compare two serialized maps
+        cbor_compare_map_eq (Map?.v v1) (Map?.v v2);
+        let f64 : squash (SZ.fits_u64) = assume (SZ.fits_u64);
+        let i1 = cbor_map_iterator_init f64 x1;
+        with p1' . assert (cbor_map_iterator_match p1' i1 (Map?.v v1));
+        unfold (cbor_map_iterator_match p1' i1 (Map?.v v1));
+        let i2 = cbor_map_iterator_init f64 x2;
+        with p2' . assert (cbor_map_iterator_match p2' i2 (Map?.v v2));
+        unfold (cbor_map_iterator_match p2' i2 (Map?.v v2));
+        let res = lex_compare_iterator_peel_perm cbor_match_map_entry cbor_serialized_map_iterator_match cbor_serialized_map_iterator_is_empty (cbor_serialized_map_iterator_next f64) cbor_compare_key_value (impl_cbor_compare_key_value ih) i1 i2;
+        fold (cbor_map_iterator_match p1' i1 (Map?.v v1));
+        fold (cbor_map_iterator_match p2' i2 (Map?.v v2));
         Trade.elim _ (cbor_match p1 x1 v1);
         Trade.elim _ (cbor_match p2 x2 v2);
         res
@@ -286,7 +315,10 @@ fn cbor_compare_body
         c
       }
     } else {
-      admit ()
+      assert (pure (ty1 == cbor_major_type_simple_value));
+      let val1 = cbor_match_simple_elim x1;
+      let val2 = cbor_match_simple_elim x2;
+      impl_uint8_compare () val1 val2
     }
   } else {
     c
